Seccap/NominalCapsule.lean
@@ -1,0 +1,267 @@
+import Seccap.Nominal
+
+namespace Term
+def value {𝔸 𝕏 C}: Term 𝔸 𝕏 C → Bool
+| const _ => true
+| abs _ e => e.ground
+| atom _ | asgn .. | unknown .. | app .. => false
+
+abbrev Value (𝔸 C) := { t : Term 𝔸 Unit C // t.value }
+abbrev Ground (𝔸 C) := { t : Term 𝔸 Unit C // t.ground }
+
+lemma value_ground {t: Term 𝔸 𝕏 C} : t.value → t.ground := by
+  induction t with simp_all [value, ground]
+
+namespace Ground
+variable {𝔸 C} (a b: 𝔸) (t t₁ t₂ : Ground 𝔸 C)
+
+abbrev atom : Ground 𝔸 C := ⟨.atom a, rfl⟩
+abbrev abs : Ground 𝔸 C := ⟨.abs a t, by simp [ground, t.2]⟩
+abbrev asgn : Ground 𝔸 C := ⟨.asgn a t, by simp [ground, t.2]⟩
+abbrev app : Ground 𝔸 C := ⟨.app t₁ t₂, by simp [ground, t₁.2, t₂.2]⟩
+abbrev const (c: C) : Ground 𝔸 C := ⟨.const c, rfl⟩
+
+abbrev swap [DecidableEq 𝔸] (h: a ≠ b) : Ground 𝔸 C := ⟨t.1.swap a b h, by simp [perm_action_ground, t.2]⟩
+
+end Ground
+
+instance {𝔸 C}: Coe (Value 𝔸 C) (Ground 𝔸 C) where
+  coe := fun ⟨t, ht⟩ => ⟨t, value_ground ht⟩
+
+variable {𝔸 𝕏 C} [DecidableEq 𝔸] {t: Term 𝔸 𝕏 C}
+
+def fvs : Term 𝔸 𝕏 C → Finset 𝔸
+| atom a => {a}
+| const .. | unknown .. => ∅
+| abs a t => t.fvs \ {a}
+| asgn a t => {a} ∪ t.fvs
+| app t₁ t₂ => t₁.fvs ∪ t₂.fvs
+
+lemma swap_fvs' {a b h x} (ha: x ≠ a) (hb: x ≠ b):
+  x ∈ t.fvs ↔ x ∈ (t.swap a b h).fvs := by
+  induction t with simp [fvs, perm_action, *] <;> simp [Perm.toEquiv, transpose] <;> grind
+
+lemma swap_fvs {a b h} :
+  t.fvs \ {a, b} = (t.swap a b h).fvs \ {a, b} := by
+  ext x
+  simp
+  apply swap_fvs'
+
+lemma fresh_fvs {a} (h : ∅ ⊢ a#t) : a ∉ t.fvs := by
+  induction h with simp [fvs, *]
+
+lemma fvs_fresh {a} (ht: t.ground) (h: a ∉ t.fvs) : ∅ ⊢ a#t := by
+  induction t with (simp [fvs] at h; simp [ground] at ht) <;> try (constructor <;> grind)
+  | abs b t ih =>
+    specialize ih ht
+    by_cases ha: a = b
+    · rw [ha]; constructor
+    · apply Fresh.F_absb
+      · exact ha
+      · apply ih
+        intro contra
+        cases ha (h contra)
+end Term
+
+def Store α β := List (α × β)
+
+namespace Store
+variable {α β} [DecidableEq α]
+
+def dom: Store α β → Finset α
+| [] => ∅
+| (a, _)::s => {a} ∪ dom s
+
+def getVal (s: Store α β) (a: α) (h: a ∈ s.dom) : β := match s with
+| (b, v)::s => if ha: a = b then v else getVal s a (by simp [dom, ha] at h; exact h)
+| [] => by simp [dom] at h
+
+def getVal? (s : Store α β) (a: α) : Option β := match s with
+| [] => none
+| (b, v)::s => if a = b then some v else getVal? s a
+
+instance : GetElem (Store α β) α β (fun s a => a ∈ s.dom) := ⟨getVal⟩
+instance : GetElem? (Store α β) α β (fun s a => a ∈ s.dom) where
+  getElem? := getVal?
+
+lemma getVal_iff_getVal? (s : Store α β) a b :
+  (∃ h, s.getVal a h = b) ↔ s.getVal? a = some b := by
+  induction s with
+  | nil => simp [dom, getVal?]
+  | cons p s ih =>
+    obtain ⟨x, y⟩ := p
+    simp [dom, getVal, getVal?]
+    split_ifs with h
+    · subst h
+      constructor
+      · intro h
+        rw [h.snd]
+      · intro h
+        simp at h
+        simp [h]
+    · constructor
+      · intro hl
+        obtain ⟨hl, hl'⟩ := hl
+        simp [h] at hl
+        apply ih.mp ⟨hl, hl'⟩
+      · intro hr
+        obtain ⟨h', hh'⟩ := ih.mpr hr
+        exact ⟨Or.inr h', hh'⟩
+
+end Store
+
+structure Capsule (𝔸 C : Type) where
+  t : Term.Ground 𝔸 C
+  σ : Store 𝔸 (Term.Value 𝔸 C)
+
+namespace Capsule
+variable {𝔸 C} [DecidableEq 𝔸]
+
+def valid (m: Capsule 𝔸 C) :=
+  m.t.1.fvs ⊆ m.σ.dom ∧ (∀ a, (h: a ∈ m.σ.dom) → (m.σ.getVal a h).1.fvs ⊆ m.σ.dom)
+
+lemma valid_app_l {t₁ t₂ : Term.Ground 𝔸 C} {σ} : valid ⟨.app t₁ t₂, σ⟩ → valid ⟨t₁, σ⟩ := by
+  obtain ⟨t₁, hg₁⟩ := t₁
+  simp [valid, Term.fvs]
+  intro h₁ h₂
+  constructor
+  · apply Finset.union_subset_left
+    exact h₁
+  · exact h₂
+
+
+lemma valid_app_r {t₁ t₂ : Term.Ground 𝔸 C} {σ} : valid ⟨.app t₁ t₂, σ⟩ → valid ⟨t₂, σ⟩ := by
+  obtain ⟨t₂, hg₂⟩ := t₂
+  simp [valid, Term.fvs]
+  intro h₁ h₂
+  constructor
+  · apply Finset.union_subset_right
+    exact h₁
+  · exact h₂
+
+lemma valid_asgn {a} {t : Term.Ground 𝔸 C} {σ} : valid ⟨t.asgn a, σ⟩ → valid ⟨t, σ⟩ := by
+  obtain ⟨t, _⟩ := t
+  simp [valid, Term.fvs]
+  rw [Finset.insert_subset_iff]
+  simp
+  intro a b c
+  simpa [b]
+
+-- read/write types with names
+-- separation/noninterference with partition σ + τ ⇒ v ∀ τ
+-- indistinguishability relation over capsules that masks part of the store
+-- inductively define store
+-- try to understand a separaation logic proof of noninterference
+-- separation for concurrency
+
+
+inductive Step [DecidableEq 𝔸] : Capsule 𝔸 C → Capsule 𝔸 C → Prop where
+| Var a σ (v: Term.Value 𝔸 C) (h: σ.getVal? a = some v): Step ⟨.atom a, σ⟩ ⟨v, σ⟩
+| App t₁ t₂ σ t₁' σ' : Step ⟨t₁, σ⟩ ⟨t₁', σ'⟩ → Step ⟨.app t₁ t₂, σ⟩ ⟨.app t₁' t₂, σ'⟩
+| AppV (v: Term.Value 𝔸 C) t₂ σ t₂' σ' : Step ⟨t₂, σ⟩ ⟨t₂', σ'⟩ → Step ⟨.app v t₂, σ⟩ ⟨.app v t₂', σ'⟩
+-- this can probably be b#t.1?
+| AppAbs a t (v: Term.Value 𝔸 C) σ b (h: b ∉ σ.dom ∪ t.1.atoms ∪ {a}) : Step ⟨.app (.abs a t) v, σ⟩ ⟨t.swap a b (by simp at h; exact Ne.symm h.left), (b, v)::σ⟩
+| Asgn a t σ t' σ' : Step ⟨t, σ⟩ ⟨t', σ'⟩ → Step ⟨.asgn a t, σ⟩ ⟨.asgn a t', σ'⟩
+| AsgnV a (v: Term.Value 𝔸 C) σ : Step ⟨.asgn a v, σ⟩ ⟨v, (a, v)::σ⟩
+
+namespace Step
+lemma dom_sub {c₁ c₂ : Capsule 𝔸 C} (h: Step c₁ c₂) : c₁.σ.dom ⊆ c₂.σ.dom := by
+  induction h with simp [*, Store.dom]
+
+lemma valid_step {c₁ c₂: Capsule 𝔸 C} (hc: c₁.valid) (h: Step c₁ c₂) : c₂.valid := by
+  induction h with
+  | Var a σ v h =>
+    simp [valid, Term.fvs] at hc
+    constructor
+    · obtain ⟨hin, heq⟩ := (σ.getVal_iff_getVal? a v).mpr h
+      simp
+      rw [← heq]
+      apply hc.right
+      exact hin
+    · simp
+      exact hc.right
+  | App t₁ t₂ σ t₁' σ' h ih =>
+    specialize ih (valid_app_l hc)
+    simp [valid, Term.fvs]
+    constructor
+    · intro a ha
+      simp at ha
+      rcases ha with ha|ha
+      · simp [valid] at ih
+        exact Finset.mem_of_subset ih.left ha
+      · simp [valid, Term.fvs] at hc
+        apply Finset.mem_of_subset _ ha
+        apply Finset.Subset.trans
+        · exact Finset.union_subset_right hc.left
+        · exact dom_sub h
+    · simp [valid] at ih
+      exact ih.right
+  | AppV v t₂ σ t₂' σ' h ih =>
+    specialize ih (valid_app_r hc)
+    simp [valid, Term.fvs]
+    simp [valid, Term.fvs] at hc
+    constructor
+    · apply Finset.union_subset
+      · apply Finset.Subset.trans _ (dom_sub h)
+        simp
+        exact Finset.union_subset_left hc.left
+      · simp [valid] at ih
+        exact ih.left
+    · simp [valid] at ih
+      exact ih.right
+  | AppAbs a t v σ b h =>
+    simp [valid]
+    constructor
+    · obtain ⟨t, ht⟩ := t
+      intro c hc'
+      simp at h
+      have hf : ∅ ⊢ b#t := t.ground_notin_atoms b ht h.right.right
+      have := t.fresh_fvs hf
+      simp [Store.dom]
+      by_cases hb: b = c
+      · simp [hb]
+      · simp [Ne.symm hb]
+        by_cases ha: a = c
+        · subst ha
+          have := t.swap_fresh a b (Ne.symm hb) _ hf ht
+          have := (mt (Term.fresh_fvs)) (not_not_intro hc')
+          contradiction
+        · rw [← t.swap_fvs'] at hc' <;> try (symm; assumption)
+          simp [valid, Term.fvs] at hc
+          grind
+    · simp [valid] at hc
+      simp [Store.dom]
+      intro c hc'
+      by_cases hb: c = b
+      · subst hb
+        simp [Store.getVal]
+        simp [Term.fvs] at hc
+        grind
+      · simp [hb] at hc'
+        simp [Store.getVal, hb]
+        have := hc.right c hc'
+        grind
+  | Asgn a t σ t' σ' h ih =>
+    specialize ih (valid_asgn hc)
+    simp [valid] at ih
+    simp [valid]
+    apply And.intro _ ih.right
+    simp [Term.fvs]
+    apply Finset.insert_subset _ ih.left
+    simp [valid, Term.fvs] at hc
+    have : a ∈ σ.dom := by grind
+    grind [dom_sub h]
+  | AsgnV a v σ =>
+    simp [valid, Store.dom]
+    simp [valid, Term.fvs] at hc
+    constructor
+    · grind
+    · intro b hb
+      by_cases ha: b = a
+      · subst ha
+        simp [Store.getVal]
+        grind
+      · simp [Store.getVal, ha]
+        grind
+end Step
+end Capsule
